debrujin

debrujin.v
@@ -5,16 +5,72 @@ Inductive LambdaTerm :=
 | app (a b: LambdaTerm)
 | abst (a: LambdaTerm).
 
-Definition s_comb := (abst (abst (abst 
-  (app (app (var 2) (var 0)) (app (var 1) (var 0)))))).
+Definition n0 := (var 0).
+Definition n1 := (var 1).
+Definition n2 := (var 2).
+Definition n3 := (var 3).
+Definition n4 := (var 4).
+Definition n5 := (var 5).
+Definition n6 := (var 6).
+
+Fixpoint lambda_eq (a b: LambdaTerm): bool :=
+match a, b with
+| var v1, var v2 => v1 =? v2
+| app a1 b1, app a2 b2 => lambda_eq a1 a2 && lambda_eq b1 b2
+| abst a1, abst a2 => lambda_eq a1 a2
+| _, _ => false
+end.
+
+Definition s_comb := (abst (abst (abst   (app (app (var 2) (var 0)) (app (var 1) (var 0)))))).
 
 Definition k_comb := (abst (abst (var 1))).
 
 (* 
+Fixpoint replace (depth: nat) (t: LambdaTerm) (r: LambdaTerm): LambdaTerm :=
+match t with
+| var n =>
+| app a b =>
+| abst b => replace (S depth) b r
+end. *)
+
+Fixpoint dec_free_vars (t: LambdaTerm) (depth: nat): LambdaTerm :=
+match t with  
+| var 0 => t
+| var (S n) => if (depth <=? n) then var n else t
+| app a b => app (dec_free_vars a depth) (dec_free_vars b depth)
+| abst a => abst (dec_free_vars a (S depth))
+end.
+
+(* depth = 0 -> 'every variable is free' *)
+(* depth = 1 -> 'every variable except 0 is free' *)
+(* depth = 2 -> 'every variable except 0, 1 is free' *)
+Fixpoint inc_free_vars (t: LambdaTerm) (depth: nat): LambdaTerm :=
+match t with
+| var n => if (depth <=? n)
+            then var (n + 1)
+            else t
+| app a b => app (inc_free_vars a depth) (inc_free_vars b depth)
+| abst a => abst (inc_free_vars a (S depth))
+end.
+
+(* starting from depth = 0 *)
+Fixpoint replace_instances (a b: LambdaTerm) (depth: nat) :=
+match a with
+| var v => if (v =? depth) 
+           then b 
+           else if (depth <? v)
+                then var (pred v)
+                else a
+| app l r => app (replace_instances l b depth) (replace_instances r b depth)
+| abst body => abst (replace_instances body b (S depth))
+end.
+
+(*
+  From Wiki:
   beta-reduction (λ M) N 
-  1. find bound instances
+  1. find bound instances in M
   2. decrement free variables of M
-  3. replace bound instances with N, incrementing free variables of N
+  3. replace bound instances of M with N, incrementing free variables of N
 
   example
    ((abst (abst (app (app (var 3) (var 1)) (abst (app (var 0) (var 2)))))) (abst (app (var 4) (var 0)))) -> 
@@ -22,66 +78,75 @@ Definition k_comb := (abst (abst (var 1))).
    (abst (app (app (var 2) (abst (app (var 5) (var 0)))) (abst (app (var 0) (abst (app (var 6) (var 0)))))))
 *)
 
-Fixpoint dec_free_vars (t: LambdaTerm) (depth: nat): LambdaTerm :=
-match t with  
-| var 0 => t
-| var (S n) => if (depth <=? n)
-               then var n
-               else t
-| app a b => app (dec_free_vars a depth) (dec_free_vars b depth)
-| abst a => abst (dec_free_vars a (S depth))
-end.
-
-Fixpoint inc_free_vars (t: LambdaTerm) (depth: nat): LambdaTerm :=
+Fixpoint beta (t: LambdaTerm): LambdaTerm :=
 match t with
-| var n => if (depth <=? n)
-            then var (S n)
-            else t
-| app a b => app (inc_free_vars a depth) (inc_free_vars b depth)
-| abst a => abst (inc_free_vars a (S depth))
+| (app (abst a) b) => (dec_free_vars (replace_instances a (inc_free_vars b 0) 0) 0)
+| app a b => let ba := beta a in
+               if (lambda_eq a ba)
+                then app a (beta b)
+                else app ba b
+| _ => t
 end.
 
-Theorem inv_fv:
+Theorem inv_fv_simple_v1:
+ forall (t: LambdaTerm) (depth: nat),
+ (dec_free_vars (inc_free_vars (var 0) depth) depth) = (var 0).
+Proof.
+ induction depth.
+  - simpl. reflexivity.
+  - simpl. reflexivity.
+Qed.
+
+Theorem inv_fv_simple_v2:
  forall (t: LambdaTerm) (depth: nat),
  (dec_free_vars (inc_free_vars t depth) depth) = t.
 Proof.
 Admitted.
 
-Example dec_example_001: dec_free_vars (var 0) 0 = (var 0).
+Example inc_000: inc_free_vars (var 0) 0 = var 1.
 Proof. simpl. reflexivity. Qed.
 
-Example inc_example_001: inc_free_vars (var 0) 0 = (var 1).
+Example inc_001: inc_free_vars (var 0) 1 = var 0.
 Proof. simpl. reflexivity. Qed.
 
-Example dec_example_002: dec_free_vars (var 1) 0 = (var 0).
+Example inc_002: inc_free_vars (var 1) 1 = var 2.
 Proof. simpl. reflexivity. Qed.
 
-Example inc_example_002: inc_free_vars (var 0) 0 = (var 1).
+Example inc_003: inc_free_vars (abst (var 0)) 0 = (abst (var 0)).
 Proof. simpl. reflexivity. Qed.
 
-Example dec_example_003: dec_free_vars (var 2) 0 = (var 1).
+Example inc_004: inc_free_vars (abst (var 1)) 0 = (abst (var 2)).
 Proof. simpl. reflexivity. Qed.
 
-Example inc_example_003: inc_free_vars (var 1) 0 = (var 2).
+Example inc_005: inc_free_vars (abst (abst (var 2))) 0 = (abst (abst (var 3))).
 Proof. simpl. reflexivity. Qed.
 
-Example dec_example_004: dec_free_vars (var 3) 0 = (var 2).
+Example inc_006: inc_free_vars (abst (abst (var 3))) 0 = (abst (abst (var 4))).
 Proof. simpl. reflexivity. Qed.
 
-Example dec_example_005: dec_free_vars (var 4) 0 = (var 3).
+Example inc_007: inc_free_vars (abst (abst (var 1))) 0 = (abst (abst (var 1))).
 Proof. simpl. reflexivity. Qed.
 
-Example dec_example_006: dec_free_vars (var 0) 1 = (var 0).
+Example inc_008: inc_free_vars (abst (abst (var 2))) 1 = (abst (abst (var 2))).
 Proof. simpl. reflexivity. Qed.
 
-Example dec_example_007: dec_free_vars (var 1) 1 = (var 1).
+Example inc_009: inc_free_vars (abst (abst (var 2))) 0 = (abst (abst (var 3))).
 Proof. simpl. reflexivity. Qed.
 
-Example dec_example_008: dec_free_vars (var 2) 1 = (var 1).
+Example beta_example_001: beta (app (abst (var 0)) (app (var 0) (var 1))) = (app (var 0) (var 1)).
 Proof. simpl. reflexivity. Qed.
 
-Example dec_example_009: dec_free_vars (var 3) 1 = (var 2).
+Example beta_example_004: 
+ beta (app (abst (abst (abst (abst ))))
+           (abst (abst (app (app n3 n1) (abst (app n0 n2)))))
+ ).
 Proof. simpl. reflexivity. Qed.
 
+Example beta_example_003: 
+ beta (app (abst (abst (app (app n3 n1) (abst (app n0 n2)))))
+           (abst (app n4 n0))) = 
+ abst (app (app n2 (abst (app n5 n0))) 
+           (abst (app n0 (abst (app n6 n0))))).
+Proof. simpl. reflexivity. Qed.
 
 
